@prefix ex: <http://example.org/ontology#> .
@prefix dbo: <https://dbpedia.org/ontology/> .
@prefix ma-ont: <http://www.w3.org/ns/ma-ont#> .
@prefix eo-ont: <https://www.eoknowledgehub.cn/eo/ontology/> .
@prefix eor: <https://www.eoknowledgehub.cn/eo/resource/> .
@prefix rdfs: <http://www.w3.org/2000/01/rdf-schema#> .
@prefix rdf: <http://www.w3.org/1999/02/22-rdf-syntax-ns#> .
@prefix owl: <http://www.w3.org/2002/07/owl#> .
@prefix schema: <http://schema.org/> .
@prefix xsd: <http://www.w3.org/2001/XMLSchema#> .

#########################
# Class Definitions
#########################

ex:NTLImage a rdfs:Class ;
    rdfs:subClassOf ma-ont:Image ;
    rdfs:label "NTL Image"@en ;
    rdfs:comment "A subclass of ma-ont:Image representing Nighttime Light images from Black Marble Dataset."@en ;
    ex:representsCounty dbo:AdministrativeRegion ;
    ex:fromSatellite eor:satellite.2011-061A ;
    ex:fromSensor eor:sensor.1c58ddb9-2b4c-4fe0-9970-f5fdc7242f6b ;
    ex:hasOutageMap ex:OutageMap .

ex:OutageMap a rdfs:Class ;
    rdfs:subClassOf ma-ont:Image ;
    rdfs:label "Outage Map"@en ;
    rdfs:comment "Power outage map of county generated using NTL Imagery and Multimodal Outage Detector."@en ;
    ex:representsCounty dbo:AdministrativeRegion .

ex:OutageRecord a rdfs:Class ;
    rdfs:label "Outage Record"@en ;
    rdfs:comment "Numerical outage record for county at date and time from Eagle-I dataset."@en ;
    ex:representsCounty dbo:AdministrativeRegion ;
    ex:hasOutageMap ex:OutageMap ;
    ex:hasNTLImage ex:NTLImage .

#########################
# Datatype Properties
#########################

ex:fipsCode a owl:DatatypeProperty ;
    rdfs:label "FIPS Code"@en ;
    schema:domainIncludes dbo:AdministrativeRegion ;
    rdfs:comment "The Federal Information Processing Standards (FIPS) code for the U.S. county."@en ;
    rdfs:range xsd:string .

ex:recordDateTime a owl:DatatypeProperty ;
    rdfs:label "Outage Record DateTime"@en ;
    schema:domainIncludes ex:OutageRecord ;
    rdfs:comment "Date and time for numerical outage record for county from Eagle-I dataset."@en ;
    rdfs:range xsd:dateTime .

ex:numberOfOutages a owl:DatatypeProperty ;
    rdfs:label "Number of Outages"@en ;
    schema:domainIncludes ex:OutageRecord ;
    rdfs:comment "Numerical outage record for county at date and time from Eagle-I dataset."@en ;
    rdfs:range xsd:integer .

#########################
# Object Properties
#########################

ex:representsCounty a owl:ObjectProperty ;
    rdfs:label "represents county"@en ;
    schema:domainIncludes ma-ont:Image , ex:OutageRecord ;
    rdfs:range dbo:AdministrativeRegion ;
    rdfs:comment "Links an NTL image, outage map, or outage record to U.S. county (instance of dbo:AdministrativeRegion) that it depicts."@en .

ex:fromSatellite a owl:ObjectProperty ;
    rdfs:label "from satellite"@en ;
    schema:domainIncludes ex:NTLImage ;
    rdfs:range eo-ont:Satellite ;
    rdfs:comment "Indicates which satellite captured the image."@en .

ex:fromSensor a owl:ObjectProperty ;
    rdfs:label "from sensor"@en ;
    schema:domainIncludes ex:NTLImage ;
    rdfs:range eo-ont:Sensor ;
    rdfs:comment "Indicates which sensor (instrument) on the satellite captured the image."@en .

ex:hasOutageMap a owl:ObjectProperty ;
    rdfs:label "has outage map"@en ;
    schema:domainIncludes ex:NTLImage , ex:OutageRecord ;
    rdfs:range ex:OutageMap ;
    rdfs:comment "Associates numerical NTL image or outage record with power outage severity map generated from NTL image."@en .

ex:hasNTLImage a owl:ObjectProperty ;
    rdfs:label "has NTL image"@en ;
    schema:domainIncludes ex:outageRecord ;
    rdfs:range ex:NTLImage ;
    rdfs:comment "Associates numerical outage record with NTL image from same day as recorded outage record."@en .